proofs/eclib/JWordExtra.ec
@@ -30,6 +30,16 @@ abstract theory WE.
   clone import BitWordSH as W with op size <- size.
   clone export BWE with op size <- size, theory BaseW <- W.
 
+  lemma to_uintUD (w1 w2: W.t) : to_uint w2 <> 0 =>
+    to_uint (w1 \udiv w2) = to_uint w1 %/ to_uint w2.
+  proof. by move=> w2_ne0; rewrite /(\udiv) /ulift2; smt(to_uint_cmp to_uint_small). qed.
+  (* FIXME: using #smt(to_uint_cmp to_uint_small) above should also work (?) *)
+
+  lemma to_uintUM (w1 w2: W.t) : 
+    to_uint (w1 \umod w2) = to_uint w1 %% to_uint w2.
+  proof. by rewrite /(\umod) /ulift2; apply to_uint_small; 
+    smt(to_uint_cmp to_uint_small JUtils.modz_cmp modz0). qed.
+
   lemma set_get (w : W.t) (i : int) : w.[i <- w.[i]] = w.
   proof. by apply/ext_eq=> j ?; rewrite get_set_if /#. qed.
 
@@ -116,6 +126,16 @@ abstract theory WE.
   rewrite sarSl // to_sint_sar1 ih.
   rewrite -divz_mulp ~-1:// 1:IntOrder.expr_gt0 ~-1://.
   by rewrite -IntID.exprSr.
+  qed.
+
+  lemma flatten_mkseq1_map_iota (f: int -> 'a) (n: int) :
+    flatten (mkseq (fun (i : int) => [f i]) n) = map f (iota_ 0 n).
+  proof.
+    elim/natind: n. smt(mkseq0 iota0).
+    move=> n n_gt0 IH. 
+    rewrite mkseqS; 1: by exact n_gt0.
+    rewrite iotaSr; 1: by exact n_gt0.
+    by rewrite flatten_rcons /= IH -cats1 map_cat map1.
   qed.
 end WE.
 
